theories/opsem/opsem.v
@@ -1,4 +1,5 @@
 Require Import basic.
+From iris.program_logic Require Import language ectx_language ectxi_language.
 
 Section opsem.
 Ltac inv H := inversion H; clear H; subst.
@@ -24,8 +25,8 @@ Ltac inv H := inversion H; clear H; subst.
     match (Δ !s! v), (Δ !s! 0) with
     | Some δ_v, Some δ_p =>
       match i with
-      | faili => ((Done Fail), ϕ)
-      | halt => ((Done Halt), ϕ)
+      | faili => ((Done FailD), ϕ)
+      | halt => ((Done HaltD), ϕ)
       | br r => (tick (upd_gen_reg Δ v PC (δ_v.gr !gr! r)) m s v v ident)
       | bne r => let Δ':= if (Z.eqb (z_of_w (δ_v.sr !sr! NZ)) 1)
                           then (upd_gen_reg Δ v PC (δ_v.gr !gr! r))
@@ -37,12 +38,12 @@ Ltac inv H := inversion H; clear H; subst.
       | ldr r1 r2 => match (valid_a δ_v r2 RE) with
                      | Some a => let Δ' :=(upd_gen_reg Δ v r1 (m !m! a)) in
                                  (tick Δ' m s v v updPC)
-                     | None => ((Done Fail), ϕ)
+                     | None => ((Done FailD), ϕ)
                      end
       | str r1 r2 => match (valid_a δ_v r1 WR) with
                      | Some a => let m' :=(upd_mem m a (δ_v.gr !gr! r2)) in
                                  (tick Δ m' s v v updPC)
-                     | None => ((Done Fail), ϕ)
+                     | None => ((Done FailD), ϕ)
                      end
       | add r1 r2 r3 => let Δ':= (upd_gen_reg Δ v r1 (w_add_w (δ_v.gr !gr! r2)(δ_v.gr !gr! r3))) in
                         (tick Δ' m s v v updPC)
@@ -58,7 +59,7 @@ Ltac inv H := inversion H; clear H; subst.
                | F_MEM_DNT => match (valid_a δ_v (nat_to_r 1) VA) with
                               | Some a => let vr :=(Z.to_nat  (z_of_w (δ_v.gr !gr! (nat_to_r 2)))) in
                                           match (Δ !s! vr) with
-                                            | Some _ => if (vr =? v) then ((Done Fail), ϕ)
+                                            | Some _ => if (vr =? v) then ((Done FailD), ϕ)
                                                         else
                                                           let pid:=(a_to_pid a) in
                                                           let s' := s ++ [(pid, vr)] in
@@ -66,18 +67,18 @@ Ltac inv H := inversion H; clear H; subst.
                                                           let Δ' := (upd_gen_reg Δ' v (nat_to_r 0) (rc_to_w SUCCESS)) in
                                                           let Δ' := (upd_gen_reg Δ' v (nat_to_r 2) (nat_to_w (length s))) in
                                                              (tick Δ' m s' v v updPC)
-                                            | None => ((Done Fail), ϕ)
+                                            | None => ((Done FailD), ϕ)
                                           end
-                              | None => ((Done Fail), ϕ)
+                              | None => ((Done FailD), ϕ)
                               end
                | F_MEM_RTRVQ => let hd := (Z.to_nat (z_of_w (δ_v.gr !gr! (nat_to_r 1)))) in
                                 match (s !! hd ) with
-                                | Some (p,v) => if (gset_elem_of_b p (δ_v.ps)) then ((Done Fail), ϕ)
+                                | Some (p,v) => if (gset_elem_of_b p (δ_v.ps)) then ((Done FailD), ϕ)
                                                 else let Δ' := (upd_ps_add Δ v p) in
                                                      let Δ' := (upd_gen_reg Δ' v (nat_to_r 0) (rc_to_w MEM_RTRVP)) in
                                                      let s' := (delete hd s) in
                                                      (tick Δ' m s' v v updPC)
-                                | _ => ((Done Fail), ϕ)
+                                | _ => ((Done FailD), ϕ)
                                 end
                | F_RUN => let vn :=(Z.to_nat  (z_of_w (δ_v.gr !gr! (nat_to_r 2)))) in
                           match (Δ !s! vn) with
@@ -90,10 +91,10 @@ Ltac inv H := inversion H; clear H; subst.
                                             let Δ' := (upd_gen_reg Δ' vn (nat_to_r 3) ws) in
                                             (tick Δ' m s v vn updPC)
                                           else (tick Δ m s v vn updPC)
-                                        | None => ((Done Fail), ϕ)
+                                        | None => ((Done FailD), ϕ)
                                         end
-                                      else ((Done Fail), ϕ)
-                          | None => ((Done Fail), ϕ)
+                                      else ((Done FailD), ϕ)
+                          | None => ((Done FailD), ϕ)
                           end
                | F_YIELD =>let Δ' := (upd_gen_reg Δ 0 (nat_to_r 0) (rc_to_w YIELD)) in
                            let Δ' := (upd_gen_reg Δ' 0 (nat_to_r 1) (nat_to_w v)) in
@@ -109,7 +110,7 @@ Ltac inv H := inversion H; clear H; subst.
                                   let Δ' := (upd_gen_reg Δ 0 (nat_to_r 0) (rc_to_w MSG_WAIT)) in
                                   let Δ' := (upd_gen_reg Δ' 0 (nat_to_r 1) (nat_to_w v)) in
                                     (tick Δ' m s v 0 updPC)
-                              | None => ((Done Fail), ϕ)
+                              | None => ((Done FailD), ϕ)
                               end
                | F_MSG_SEND =>match δ_v.π.1 with
                               | Some (pt) =>
@@ -129,29 +130,29 @@ Ltac inv H := inversion H; clear H; subst.
                                                    | Some (((pr, false), _), _) =>
                                                      let Δ' := (upd_gen_reg Δ v (nat_to_r 0) (rc_to_w BUSY)) in
                                                      (tick Δ' m s v v updPC)
-                                                   | None => ((Done Fail), ϕ)
+                                                   | None => ((Done FailD), ϕ)
                                                    end
-                                    | None => ((Done Fail), ϕ)
+                                    | None => ((Done FailD), ϕ)
                                   end
-                                else ((Done Fail), ϕ)
-                              | None => ((Done Fail), ϕ)
+                                else ((Done FailD), ϕ)
+                              | None => ((Done FailD), ϕ)
                               end
                | F_MSG_RCV => match δ_v.π.2 with
                               | Some (((pr, b), ws), vs) =>
                                 if b then
                                   let Δ' := (upd_rx Δ v (Some (((pr, false), ws), v))) in
                                   (tick Δ' m s v v updPC)
-                                else ((Done Fail), ϕ)
-                              | _ => ((Done Fail), ϕ)
+                                else ((Done FailD), ϕ)
+                              | _ => ((Done FailD), ϕ)
                               end
-               | F_UNKNOWN =>((Done Fail), ϕ)
+               | F_UNKNOWN =>((Done FailD), ϕ)
                end
       | mrs r1 r2 =>  let Δ':= (upd_gen_reg Δ v r1 (δ_v.sr !sr! r2)) in
                     (tick Δ' m s v v updPC)
       | msr r1 r2 =>  let Δ':= (upd_sys_reg Δ v r1 (δ_v.gr !gr! r2)) in
                     (tick Δ' m s v v updPC)
       end
-    | _,_ => ((Done Fail), ϕ)
+    | _,_ => ((Done FailD), ϕ)
     end.
  (* valid_a = Some a is better *)
 (* Inductive isValidPC: list State -> VMID -> Prop :=
@@ -184,12 +185,12 @@ Inductive step: Conf → Conf → Prop :=
   | step_exec_invalid_vmid:
       forall ϕ v,
         (ϕ.1 !s! v) = None->
-        step ((ExecInstr v), ϕ) ((Done Fail), ϕ)
+        step ((ExecInstr v), ϕ) ((Done FailD), ϕ)
   | step_exec_invalid_pc:
       forall ϕ v δ,
         (ϕ.1 !s! v) =Some δ ->
         (valid_a δ PC VA)=None ->
-        step ((ExecInstr v), ϕ) ((Done Fail), ϕ)
+        step ((ExecInstr v), ϕ) ((Done FailD), ϕ)
   | step_exec_instr:
       forall ϕ v δ a i,
         (ϕ.1 !s! v) =Some δ ->
@@ -205,11 +206,11 @@ Lemma normal_always_step:
     - destruct  (valid_a s PC VA) eqn:Ha.
       + destruct (exec (decodeInstr ((ϕ.m) !m! a)) ϕ v) eqn:He.
         exists e, e0. rewrite <-He. eapply step_exec_instr; eauto.
-      + exists (Done Fail), ϕ.
+      + exists (Done FailD), ϕ.
         eapply step_exec_invalid_pc.
         done.
         assumption.
-    - exists (Done Fail), ϕ.
+    - exists (Done FailD), ϕ.
       eapply step_exec_invalid_vmid.
       assumption.
 Qed.
@@ -250,7 +251,7 @@ Qed.
   Lemma step_invalid_vmid_fail_inv (Δ : list State) (m:Mem)  (s: ShareStates)v c (ϕ': ExecConf) :
     (Δ !s! v)= None ->
     step ((ExecInstr v) ,(Δ, (m,s))) (c, ϕ') ->
-    c = (Done Fail) ∧ ϕ' = (Δ, (m,s)).
+    c = (Done FailD) ∧ ϕ' = (Δ, (m,s)).
   Proof.
     intros.
    inv H1.
@@ -263,10 +264,187 @@ Qed.
      inv H5.
   Qed.
 
-  (*TODO: step_invalid_pc_fail_inv*)
+  (*TODO: step_invalid_pc_fail_inv, skip it for now*)
 
-    (*TODO:val*)
+    (*val*)
+ Inductive val: Type :=
+  | HaltedV: val
+  | FailedV: val
+  | NextIV (v: VMID): val.
 
-    (*TODO:expr*)
+  Inductive expr: Type :=
+  | Single (m : ExecMode)
+  | Repeat (e : expr).
+
+  Definition state : Type := ExecConf.
+
+  Definition of_val (v: val): expr :=
+    match v with
+    | HaltedV => (Single (Done HaltD))
+    | FailedV => (Single (Done FailD))
+    | NextIV n => (Single (Done (NextD n)))
+    end.
+
+  Definition to_val (e: expr): option val :=
+    match e with
+    | Single d=>
+      match d with
+      | Done HaltD => Some HaltedV
+      | Done FailD => Some FailedV
+      | Done (NextD n) => Some (NextIV n)
+      | ExecInstr _ => None
+      end
+    | Repeat _ => None
+    end.
+
+  Lemma of_to_val:
+    forall e v, to_val e = Some v →
+           of_val v = e.
+  Proof.
+    intros * HH.
+    destruct e;try (destruct m;simpl in HH;inv HH).
+    destruct d;simpl in H1;inv H1;simpl;done.
+    inv HH.
+  Qed.
+
+  Lemma to_of_val:
+    forall v, to_val (of_val v) = Some v.
+  Proof. destruct v; reflexivity. Qed.
+
+(*Evaluation context*)
+  Inductive ectx_item :=
+  | RepeatCtx.
+
+  Notation ectx := (list ectx_item).
+
+  Definition fill_item (Ki : ectx_item) (e : expr) : expr :=
+    match Ki with
+    | RepeatCtx => Repeat e
+    end.
+
+  (*reduction rules *)
+  (* TODO: remove Single *)
+  Inductive prim_step: expr → state → list Empty_set → expr → state → list expr → Prop :=
+  | PS_no_fork_single n σ e' σ' :
+      step ((ExecInstr n), σ) (e', σ') → prim_step (Single (ExecInstr n)) σ [] (Single e') σ' []
+  | PS_no_fork_next n σ : prim_step (Repeat (Single (Done (NextD n)))) σ [] (Repeat (Single (ExecInstr n))) σ []
+  | PS_no_fork_halt σ : prim_step (Repeat (Single (Done HaltD))) σ [] (Single (Done HaltD)) σ []
+  | PS_no_fork_fail σ : prim_step (Repeat (Single (Done FailD))) σ [] (Single (Done FailD)) σ [].
+
+  Lemma val_stuck:
+    forall e σ o e' σ' efs,
+      prim_step e σ o e' σ' efs →
+      to_val e = None.
+  Proof. intros * HH. by inversion HH. Qed.
+
+  Lemma prim_step_exec_inv n σ1 l1 e2 σ2 efs :
+    prim_step (Single (ExecInstr n)) σ1 l1 e2 σ2 efs →
+    l1 = [] ∧ efs = [] ∧
+    exists (c: ExecMode),
+      e2 = (Single c)∧
+      step ((ExecInstr n ), σ1) (c, σ2).
+  Proof. inversion 1; subst; split; eauto. Qed.
+
+  Lemma prim_step_and_step_exec n σ1 e2 σ2 l1 e2' σ2' efs :
+    step ((ExecInstr n), σ1) (e2, σ2) →
+    prim_step (Single (ExecInstr n)) σ1 l1 e2' σ2' efs →
+    l1 = [] ∧ e2' = (Single e2) ∧ σ2' = σ2 ∧ efs = [].
+  Proof.
+    intros* Hstep Hpstep.
+    inversion Hpstep as [? ? ? ? Hstep' | | |]; subst.
+    generalize (step_deterministic _ _ _ _ _ _ Hstep Hstep'). intros [-> ->].
+    auto.
+  Qed.
+
+  Lemma vm_lang_determ e1 σ1 κ κ' e2 e2' σ2 σ2' efs efs' :
+    prim_step e1 σ1 κ e2 σ2 efs →
+    prim_step e1 σ1 κ' e2' σ2' efs' →
+    κ = κ' ∧ e2 = e2' ∧ σ2 = σ2' ∧ efs = efs'.
+  Proof.
+    intros Hs1 Hs2. inv Hs1; inv Hs2.
+    all: repeat match goal with HH : step _ _ |- _ => inv HH end; try congruence.
+    all: auto.
+    rewrite H5 in H7; inv H7.
+    rewrite H8 in H6; inv H6.
+    rewrite H3 in H4; inv H4.
+    done.
+  Qed.
+
+  Lemma fill_item_val Ki e :
+    is_Some (to_val (fill_item Ki e)) → is_Some (to_val e).
+  Proof. intros [v ?]. destruct Ki; simplify_option_eq; eauto. Qed.
+  Instance fill_item_inj Ki : Inj (=) (=) (fill_item Ki).
+  Proof. destruct Ki; intros ???; simplify_eq; auto with f_equal. Qed.
+  Lemma head_ctx_step_val Ki e σ1 κ e2 σ2 ef :
+    prim_step (fill_item Ki e) σ1 κ e2 σ2 ef → is_Some (to_val e).
+  Proof. destruct Ki; inversion_clear 1; simplify_option_eq; eauto. Qed.
+  Lemma fill_item_no_val_inj Ki1 Ki2 e1 e2 :
+    to_val e1 = None → to_val e2 = None →
+    fill_item Ki1 e1 = fill_item Ki2 e2 → Ki1 = Ki2.
+  Proof.
+    destruct Ki1, Ki2; intros; try discriminate; simplify_eq;
+    repeat match goal with
+           | HH : to_val (of_val _) = None |- _ => by rewrite to_of_val in HH
+           end; auto.
+  Qed.
+  Lemma vm_lang_mixin : EctxiLanguageMixin of_val to_val fill_item prim_step.
+    constructor.
+    apply to_of_val.
+    apply of_to_val.
+    apply val_stuck.
+    apply fill_item_val.
+    apply fill_item_inj.
+    apply fill_item_no_val_inj.
+    apply head_ctx_step_val.
+Qed.
+
+ Definition is_atomic (e : expr) : Prop :=
+    match e with
+    | Single _ => True
+    | _ => False
+    end.
+ (* ugly proofs... *)
+ Lemma tick_updpc_atomic Δ m s n v :
+   ∃ v' ϕ', (tick Δ m s n v updPC) = ((Done FailD), ϕ') ∨
+         ((tick Δ m s n v updPC) = ((Done (NextD v') ,ϕ'))) ∨
+          ((tick Δ m s  n v updPC)= ((Done HaltD) ,ϕ')).
+  Proof.
+    rewrite /tick; rewrite /updPC;
+      repeat case_match.
+     exists 0; eauto.
+     exists 0; eauto.
+     exists v; eauto.
+     exists v; eauto.
+     exists 0; eauto.
+     exists 0; eauto.
+  Qed.
+
+  Lemma tick_id_atomic Δ m s n v:
+   ∃ v' ϕ', (tick Δ m s n v ident) = ((Done FailD), ϕ') ∨
+         ((tick Δ m s n v ident) = ((Done (NextD v') ,ϕ'))) ∨
+          ((tick Δ m s n v ident)= ((Done HaltD) ,ϕ')).
+  Proof.
+    rewrite /tick; rewrite /ident;
+      repeat case_match.
+     exists 0; eauto.
+     exists v; eauto.
+     exists 0; eauto.
+     exists 0; eauto.
+  Qed.
+
+  Lemma instr_atomic i φ n :
+    ∃ n' φ', (exec i φ n = ((Done FailD), φ')) ∨ (exec i φ n = ((Done (NextD n')), φ')) ∨
+          (exec i φ n = ((Done HaltD), φ')).
+  Proof.
+    unfold exec.
+    repeat case_match;
+      try (apply tick_updpc_atomic);
+      try (apply tick_id_atomic);
+      try (exists 0; eauto).
+    Qed.
 
 End opsem.
+
+Canonical Structure vm_ectxi_lang `{InstrEncoding} := EctxiLanguage vm_lang_mixin.
+Canonical Structure vm_ectx_lang `{InstrEncoding} := EctxLanguageOfEctxi vm_ectxi_lang.
+Canonical Structure vm_lang `{InstrEncoding} := LanguageOfEctx vm_ectx_lang.
